

$$a^2 + b^2 = c^2$$

$$x = \frac{-b \pm \sqrt{b^2 - 4ac}}{2a}$$

$$v = \frac{d}{t}$$

$$F = ma$$

$$\rho = \frac{m}{V}$$

$$m = \frac{y_2 - y_1}{x_2 - x_1}$$

$$V = IR$$

$$V = \frac{4}{3} \pi r^3$$

$$K = \frac{1}{2}mv^2$$

$$p = mv$$

$$PV = nRT$$

$$|a + b| \leq |a| + |b|$$

$$\text{pH} = -\log_{10} [H^+]$$

$$F = k \frac{q_1 q_2}{r^2}$$

$$n_1 \sin \theta_1 = n_2 \sin \theta_2$$

$$P(A \mid B) = \frac{P(B \mid A) P(A)}{P(B)}$$

$$F = G \frac{m_1 m_2}{r^2}$$

$$F = kx$$

$$\Delta G = \Delta H - T \Delta S$$

$$\Delta S_{\text{univ}} \geq 0$$

$$\int_a^b f'(x) \, dx = f(b) - f(a)$$

$$E = mc^2$$

$$A = Pe^{rt}$$

$$f(x) = \frac{1}{\sigma\sqrt{2\pi}} e^{-\frac{(x-\mu)^2}{2\sigma^2}}$$

$$(x + y)^n = \sum_{k=0}^n \binom{n}{k} x^{n-k} y^k$$

$$\hat{f}(\xi) = \int_{-\infty}^{\infty} f(x) e^{-2\pi i x \xi} dx$$

$$\nabla \cdot \mathbf{E} = \rho/\epsilon_0$$

$$\nabla \times \mathbf{E} = - \frac{\partial \mathbf{B}}{\partial t}$$

$$\rho\left(\frac{\partial \mathbf{u}}{\partial t} + (\mathbf{u} \cdot \nabla)\mathbf{u}\right) = -\nabla p + \mu \nabla^2 \mathbf{u}$$

$$e^{i\pi} + 1 = 0$$

$$|\langle u, v \rangle| \leq |u| |v|$$